ulib/FStar.Tactics.Logic.fst
@@ -212,9 +212,19 @@ private val __and_elim : (#p:Type) -> (#q:Type) -> (#phi:Type) ->
                               Lemma phi
 let __and_elim #p #q #phi p_and_q f = ()
 
-let and_elim (t : term) : Tac unit =
-    let ae = `__and_elim in
-    apply_lemma (mk_e_app ae [t])
+private val __and_elim' : (#p:Type) -> (#q:Type) -> (#phi:Type) ->
+                              squash (p /\ q) ->
+                              squash (p ==> q ==> phi) ->
+                              Lemma phi
+let __and_elim' #p #q #phi p_and_q f = ()
+
+let and_elim (t : term) : Tac (binder * binder) =
+    begin
+     try apply_lemma (`(__and_elim (`#t)))
+     with | _ -> apply_lemma (`(__and_elim' (`#t)))
+    end;
+    (implies_intro (), implies_intro ())
+
 
 private val __witness : (#a:Type) -> (x:a) -> (#p:(a -> Type)) -> squash (p x) -> squash (l_Exists p)
 private let __witness #a x #p _ =
