ulib/FStar.Tactics.PatternMatching.fst
@@ -143,7 +143,7 @@ let repeat' #a (f: unit -> Tac a) : Tac unit =
   let _ = repeat f in ()
 
 let and_elim' (h: binder) : Tac unit =
-  and_elim (pack (Tv_Var (bv_of_binder h)));
+  let _ = and_elim (pack (Tv_Var (bv_of_binder h))) in
   clear h
 
 (** Use a hypothesis at type a to satisfy a goal at type squash a *)
